dev/lf/doc.md
@@ -16,13 +16,13 @@ Here is [the corresponding Coq script](dot_top_bot.v).
                        {A: S..T}                    type declaration
                        S & T                        intersection
                        x.A                          projection
-                       rec(x: T)                    recursive dependent type
-                       all(x: S)T                   dependent function
+                       μ(x: T)                    recursive dependent type
+                       ∀(x: S)T                     dependent function
                        Top                          top type
                        Bot                          bottom type
 
     Value          v = new(x: T)d                   object
-                       lambda(x: T)t                lambda
+                       λ(x: T)t                     lambda
 
     Term     s, t, u = x                            variable
                        v                            value
@@ -35,7 +35,7 @@ Here is [the corresponding Coq script](dot_top_bot.v).
                        d & d'                       aggregate definition
 
     Store          s = ... x = v ...
-    Environment    G = ... x: T ...
+    Environment    Γ = ... x: T ...
 
 ***
 
@@ -44,7 +44,7 @@ Here is [the corresponding Coq script](dot_top_bot.v).
     (Project)
                              s | x.a  -->  s | t          if s(x) = new(x: T)(d, a = t)
     (Apply)
-                             s | x y  -->  s | [z:=y]t    if s(x) = lambda(z: T)t
+                             s | x y  -->  s | [z:=y]t    if s(x) = λ(z: T)t
     (Let-Var)
                   s | let x = y in t  -->  s | [x:=y]t
     (Let-Value)
@@ -58,108 +58,108 @@ Here is [the corresponding Coq script](dot_top_bot.v).
 
 ## Typing Rules
 
-### Type Assignment `G |- t: T`
+### Type Assignment `Γ ⊢ t: T`
 
     (Var)
-                            G, x: T, G' |- x: T
+                            Γ, x: T, Γ' ⊢ x: T
     (All-I)
-                       G, x: T |- t: U    (x not in fv(T))
+                       Γ, x: T ⊢ t: U    (x ∉ fv(T))
                        -----------------------------------
-                          G |- lambda(x: T)t: all(x: T)U
+                          Γ ⊢ λ(x: T)t: ∀(x: T)U
     (All-E)
-                       G |- x: all(z: S)T    G |- y: S
+                       Γ ⊢ x: ∀(z: S)T    Γ ⊢ y: S
                        -------------------------------
-                              G |- x y: [z:=y]T
+                              Γ ⊢ x y: [z:=y]T
     ({}-I)
-                               G, x: T |- d: T
+                               Γ, x: T ⊢ d: T
                           --------------------------
-                          G |- new(x: T)d: rec(x: T)
+                          Γ ⊢ new(x: T)d: μ(x: T)
     ({}-E)
-                                G |- x: {a: T}
+                                Γ ⊢ x: {a: T}
                                 --------------
-                                 G |- x.a: T
+                                 Γ ⊢ x.a: T
     (Let)
-                G |- t: T   G, x: T |- u: U   (x not in fv(U))
+                Γ ⊢ t: T   Γ, x: T ⊢ u: U   (x ∉ fv(U))
                 ----------------------------------------------
-                            G |- let x = t in u: U
+                            Γ ⊢ let x = t in u: U
     (Rec-I)
-                                  G |- x: T
+                                  Γ ⊢ x: T
                               -----------------
-                              G |- x: rec(x: T)
+                              Γ ⊢ x: μ(x: T)
     (Rec-E)
-                              G |- x: rec(x: T)
+                              Γ ⊢ x: μ(x: T)
                               -----------------
-                                  G |- x: T
+                                  Γ ⊢ x: T
     (&-I)
-                            G |- x: T   G |- x: U
+                            Γ ⊢ x: T   Γ ⊢ x: U
                             ---------------------
-                                G |- x: T & U
+                                Γ ⊢ x: T & U
     (Sub)
-                           G |- t: T   G |- T <: U
+                           Γ ⊢ t: T   Γ ⊢ T <: U
                            -----------------------
-                                  G |- t: U
+                                  Γ ⊢ t: U
 
 ***
 
-### Definition Type Assignment `G |- d: T`
+### Definition Type Assignment `Γ ⊢ d: T`
 
     (Fld-I)
-                                  G |- t: T
+                                  Γ ⊢ t: T
                              --------------------
-                             G |- {a = t}: {a: T}
+                             Γ ⊢ {a = t}: {a: T}
     (Typ-I)
-                           G |- {A = T}: {A: T..T}
+                           Γ ⊢ {A = T}: {A: T..T}
     (AndDef-I)
-           G |- d1: T1   G |- d2: T2   (dom(d1), dom(d2) disjoint)
+           Γ ⊢ d1: T1   Γ ⊢ d2: T2   (dom(d1), dom(d2) disjoint)
            -------------------------------------------------------
-                            G |- d1 & d2: T1 & T2
+                            Γ ⊢ d1 & d2: T1 & T2
 
 
 ***
 
-### Subtyping: `G |- T <: U`
+### Subtyping: `Γ ⊢ T <: U`
 
     (<:-Top)
-                                G |- T <: Top
+                                Γ ⊢ T <: Top
     (Bot-<:)
-                                G |- Bot <: T
+                                Γ ⊢ Bot <: T
     (Refl-<:)
-                                G |- T <: T
+                                Γ ⊢ T <: T
     (Trans-<:)
-                          G |- S <: T   G |- T <: U
+                          Γ ⊢ S <: T   Γ ⊢ T <: U
                           -------------------------
-                                 G |- S <: U
+                                 Γ ⊢ S <: U
     (And-<:)
-                               G |- T & U <: T
+                               Γ ⊢ T & U <: T
 
-                               G |- T & U <: U
+                               Γ ⊢ T & U <: U
     (<:-And)
-                          G |- S <: T   G |- S <: U
+                          Γ ⊢ S <: T   Γ ⊢ S <: U
                           -------------------------
                                   S <: T & U
     (Fld-<:-Fld)
-                                 G |- T <: U
+                                 Γ ⊢ T <: U
                             ---------------------
-                            G |- {a: T} <: {a: U}
+                            Γ ⊢ {a: T} <: {a: U}
     (Typ-<:-Typ)
-                        G |- S2 <: S1   G |- T1 <: T2
+                        Γ ⊢ S2 <: S1   Γ ⊢ T1 <: T2
                        -------------------------------
-                       G |- {A: S1..T1} <: {A: S2..T2}
+                       Γ ⊢ {A: S1..T1} <: {A: S2..T2}
     (<:-Sel)
-                              G |- x: {A: S..T}
+                              Γ ⊢ x: {A: S..T}
                               -----------------
-                                G |- S <: x.A
+                                Γ ⊢ S <: x.A
     (Sel-<:)
-                              G |- x: {A: S..T}
+                              Γ ⊢ x: {A: S..T}
                               -----------------
-                               G |- x.A <: T
+                               Γ ⊢ x.A <: T
     (All-<:-All)
-                     G |- S2 <: S1   G, x: S2 |- T1 <: T2
+                     Γ ⊢ S2 <: S1   Γ, x: S2 ⊢ T1 <: T2
                      ------------------------------------
-                      G |- all(x: S1)T1 <: all(x: S2)T2
+                      Γ ⊢ ∀(x: S1)T1 <: ∀(x: S2)T2
 
 
-*Note:* `G, x: T` is well-defined only if `x` is neither in the domain of `G` nor in
+*Note:* `Γ, x: T` is well-defined only if `x` is neither in the domain of `Γ` nor in
 its free variables.
 
 ***
@@ -179,11 +179,11 @@ Allow terms in applications and selections, using the expansions
 
 Expand type ascriptions to applications:
 
-                         t: T  ===  (lambda(x: T)x)t
+                         t: T  ===  (λ(x: T)x)t
 
 Shorthand syntax for object types and values:
 
-         { z => D1; ...; Dn }  ===  rec(z: D1 & ... & Dn)
+         { z => D1; ...; Dn }  ===  μ(z: D1 & ... & Dn)
      new { z => d1; ...; dn }  ===  new(x: D1 & ... & Dn)d1 & ... & dn
                                     where Di derived from di. (di needs to have full type info)
 
@@ -202,13 +202,13 @@ Shorthand syntax for self bounds: In type of `x`, expand
     let scala_units =
       let scala_units_impl =
         new (su:
-              { Unit: all(x: su.Unit)su.Unit..all(x: su.Unit)su.Unit } &
+              { Unit: ∀(x: su.Unit)su.Unit..∀(x: su.Unit)su.Unit } &
               { unit: su.Unit }
-            ) { Unit = all(x: su.Unit)su.Unit } &
-              { unit = lambda(x: su.Unit)x }
+            ) { Unit = ∀(x: su.Unit)su.Unit } &
+              { unit = λ(x: su.Unit)x }
       in let scala_units_api_wrapper =
-        lambda(x:
-          { a: rec(su:
+        λ(x:
+          { a: μ(su:
                     { Unit: su.Unit..su.Unit } &
                     { unit: su.Unit }
                   )
@@ -220,11 +220,11 @@ Or, using some of the shorthands:
 
     let scala_units =
       new (su: {
-        Unit: all(x: su.Unit)su.Unit .. all(x: su.Unit)su.Unit
+        Unit: ∀(x: su.Unit)su.Unit .. ∀(x: su.Unit)su.Unit
         unit: su.Unit
       }) {
-        Unit = all(x: su.Unit)su.Unit
-        unit = lambda(x: su.Unit)x
+        Unit = ∀(x: su.Unit)su.Unit
+        unit = λ(x: su.Unit)x
       }: { su =>
         Unit: su.Unit .. su.Unit
         unit: su.Unit
@@ -234,8 +234,8 @@ Or, even shorter:
 
     let scala_units =
       new { su =>
-        Unit = all(x: su.Unit)su.Unit
-        unit: su.Unit = lambda(x: su.Unit)x
+        Unit = ∀(x: su.Unit)su.Unit
+        unit: su.Unit = λ(x: su.Unit)x
       }: { su =>
         Unit
         unit: su.Unit
@@ -246,18 +246,18 @@ Encoding a generic list type:
     let scala_collections_immutable =
       new { sci =>
         List = { thisList => A; head: thisList.A; tail: sci.List & { A = thisList.A } }
-        nil: all(x: {A})sci.List & {A = x.A} =
-          lambda(x: {A})
+        nil: ∀(x: {A})sci.List & {A = x.A} =
+          λ(x: {A})
             let thisList = new { thisList => A = x.A; head = thisList.head; tail = thisList.tail }
             in thisList
-        cons: all(x: {A})all(hd: x.A)all(tl: sci.List & {A = x.A})sci.List & {A = x.A} =
-          lambda(x: {A})lambda(hd: x.A)lambda(tl: sci.List & {A = x.A})
+        cons: ∀(x: {A})∀(hd: x.A)∀(tl: sci.List & {A = x.A})sci.List & {A = x.A} =
+          λ(x: {A})λ(hd: x.A)λ(tl: sci.List & {A = x.A})
              let thisList = new { thisList => A = x.A; head = hd; tail = tl }
              in thisList
       }: { sci =>
         List <: { thisList => A; head: thisList.A; tail: sci.List & { A = thisList.A } }
-        nil: all(x: {A})sci.List & {A = x.A}
-        cons: all(x: {A})all(hd: x.A)all(tl: sci.List & {A = x.A})sci.List & {A = x.A}
+        nil: ∀(x: {A})sci.List & {A = x.A}
+        cons: ∀(x: {A})∀(hd: x.A)∀(tl: sci.List & {A = x.A})sci.List & {A = x.A}
       }
 
 Here's a detailed argument why the body of the `cons` method has the required type
@@ -265,7 +265,7 @@ Here's a detailed argument why the body of the `cons` method has the required ty
 
 (1) We have:
 
-       thisList: rec(thisList: { A = x.A, hd: x.A, tl: sci.List & {A = x.A}})
+       thisList: μ(thisList: { A = x.A, hd: x.A, tl: sci.List & {A = x.A}})
 
             by (Rec-E)
 
@@ -281,10 +281,10 @@ Here's a detailed argument why the body of the `cons` method has the required ty
 
              by (Rec-I)
 
-       thisList: rec(thisList: { A, hd: thisList.A, tl: sci.List & { A = thisList.A}})
+       thisList: μ(thisList: { A, hd: thisList.A, tl: sci.List & { A = thisList.A}})
 
              by (Sub), since
-             rec(thisList: { A, hd: thisList.A, tl: sci.List & { A = thisList.A}})
+             μ(thisList: { A, hd: thisList.A, tl: sci.List & { A = thisList.A}})
                <: sci.List
 
        thisList: sci.List
@@ -319,7 +319,7 @@ Generally, we can encode:
 
 ### Definition (Precise typing)
 
-`G |-! t: T` if `G |- t: T` and the following two conditions hold:
+`Γ ⊢! t: T` if `Γ ⊢ t: T` and the following two conditions hold:
 
  1. If `t` is a value, the typing derivation of `t` ends in (All-I) or ({}-I).
  2. If `t` is a variable, the typing derivation of `t` consists only of (Var), (Rec-E)
@@ -328,201 +328,201 @@ Generally, we can encode:
 
 ### Definition (Environment/store correspondence)
 
-An environment `G` corresponds to a store `s`, written `G ~ s`, if `G ~ s` can be derived
+An environment `Γ` corresponds to a store `s`, written `Γ ~ s`, if `Γ ~ s` can be derived
 using the rules below.
 
                               (empty) ~ (empty)
 
-                              G ~ s   G |-! v: T
+                              Γ ~ s   Γ ⊢! v: T
                               ------------------
-                              G, x: T ~ s, x = v
+                              Γ, x: T ~ s, x = v
 
 ### Definition (Underlying value)
 Given a store `s` and a variable `x` bound in `s`,
 the underlying value `s(x)` is the value `v` such that `x = v in s`.
 
 ### Lemma (Weakening)
-Let `G = G', x: S`. Then
+Let `Γ = Γ', x: S`. Then
 
- - If `G' |- t: T` then `G |- t: T`
- - If `G' |-! v: T` then `G |-! v: T`.
- - If `G' |- T <: U` then `G |- T <: U`.
- - If `G' ~ s` then `G ~ s`.
+ - If `Γ' ⊢ t: T` then `Γ ⊢ t: T`
+ - If `Γ' ⊢! v: T` then `Γ ⊢! v: T`.
+ - If `Γ' ⊢ T <: U` then `Γ ⊢ T <: U`.
+ - If `Γ' ~ s` then `Γ ~ s`.
 
 *Proof*: All derivations remain valid in an environment with extra information.
 
 ### Definition (Environment subsumption)
 
-Environment `G` subsumes `G'`, written `G <: G'`, if
-for all `x: T` in `G'` we have `G |- x: T`.
+Environment `Γ` subsumes `Γ'`, written `Γ <: Γ'`, if
+for all `x: T` in `Γ'` we have `Γ ⊢ x: T`.
 
 
 ### Lemma (Narrowing)
 
-If `G <: G'` then:
+If `Γ <: Γ'` then:
 
- - If `G' |- t: T` then also `G |- t: T`
- - If `G' |- d: T` then also `G |- d: T`
- - If `G' |- S <: T` then also `G' |- S <: T`
+ - If `Γ' ⊢ t: T` then also `Γ ⊢ t: T`
+ - If `Γ' ⊢ d: T` then also `Γ ⊢ d: T`
+ - If `Γ' ⊢ S <: T` then also `Γ' ⊢ S <: T`
 
 *Proof*: A straightforward induction on typing, subtyping and well-formedness derivations.
 
 
 ### Definition (Environment Renaming)
 
-    [x:=y]G = [[x:=y]z: [x:=y]T | z: T in G]
+    [x:=y]Γ = [[x:=y]z: [x:=y]T | z: T in Γ]
 
 ### Lemma (Renaming)
 Let [s] be a renaming `[x0:=y0]` for arbitrary variables `x0`, `y0`. Then
 
- - `     [s]rec(x: T)  =  rec([s]x: [s]T)`
- - `    [s]all(x: T)U  =  all([s]x: [s]T): [s]U`
+ - `     [s]μ(x: T)  =  μ([s]x: [s]T)`
+ - `    [s]∀(x: T)U  =  ∀([s]x: [s]T): [s]U`
  - `    [s]new(x: T)d  =  new([s]x: [s]T): [s]d`
- - ` [s]lambda(x: T)t  =  lambda([s]x: [s]T): [s]t`
+ - ` [s]λ(x: T)t  =  λ([s]x: [s]T): [s]t`
  - `[s]let x = t in u  =  let [s]x = [s]t in [s]u`
 
 *Proof*. We prove the first equation; the others are analogous. We distinguish whether or not `x0 = x`.
 
 If `x0 = x` then
 
-      [s]rec(x0: T)
+      [s]μ(x0: T)
     = (by definition of substitution)
-      rec(x0: T)
+      μ(x0: T)
     = (by alpha renaming x0 to y0)
-      rec(y0: [y0:=x0]T)
+      μ(y0: [y0:=x0]T)
     = (by rewriting)
-      rec([s]x0: [s]T)
+      μ([s]x0: [s]T)
 
 If `x0 != x` then
 
-      [s]rec(x: T)
+      [s]μ(x: T)
     = (by definition of substitution)
-      rec(x: [s]T)
+      μ(x: [s]T)
     = (since x0 != x)
-      rec([s]x0: [s]T)
+      μ([s]x0: [s]T)
 
 ### Lemma (Subst)
- 1. If `G, x: S |- t: T` and `G |- y: [x:=y]S`
-then `G |- [x:=y]t: [x:=y]T`.
- 2. If `G, x: S |- d: T` and `G |- y: [x:=y]S`
-then `G |- [x:=y]d: [x:=y]T`.
+ 1. If `Γ, x: S ⊢ t: T` and `Γ ⊢ y: [x:=y]S`
+then `Γ ⊢ [x:=y]t: [x:=y]T`.
+ 2. If `Γ, x: S ⊢ d: T` and `Γ ⊢ y: [x:=y]S`
+then `Γ ⊢ [x:=y]d: [x:=y]T`.
 
 We prove the more general proposition:
 
-If `G, x: S, G' |- t: T` and `G, [x:=y]G' |- y: [x:=y]S`, then
-`G, [x:=y]G' |- [x:=y]t: [x:=y]T`. (and the same for `d` instead of `t`).
+If `Γ, x: S, Γ' ⊢ t: T` and `Γ, [x:=y]Γ' ⊢ y: [x:=y]S`, then
+`Γ, [x:=y]Γ' ⊢ [x:=y]t: [x:=y]T`. (and the same for `d` instead of `t`).
 
 Proof by mutual induction on derivations.
 Let `[s] = [x0:=y0]`.
-Assume `G, x0: S0, G' |- t0: T0` and `G, [s]G' |- y0: [s]S0`.
-To show: `G, [s]G' |- [s]t0: [s]T0`.
+Assume `Γ, x0: S0, Γ' ⊢ t0: T0` and `Γ, [s]Γ' ⊢ y0: [s]S0`.
+To show: `Γ, [s]Γ' ⊢ [s]t0: [s]T0`.
 
-We distinguish according to the last rule in the derivation of `G, x0: S0, G' |- t0: T0`
+We distinguish according to the last rule in the derivation of `Γ, x0: S0, Γ' ⊢ t0: T0`
 
 **Case (Var)**: We have in this case: `t = x0`, `T0 = S0`,
-`G, x0: S0, G' |- x: S0`, and `G, [s]G' |- y0: [s]S0`.
-Together, `G, x0: S0, G' |- [s]x0: [s]S0`.
+`Γ, x0: S0, Γ' ⊢ x: S0`, and `Γ, [s]Γ' ⊢ y0: [s]S0`.
+Together, `Γ, x0: S0, Γ' ⊢ [s]x0: [s]S0`.
 
-**Case (All-I)** Then `t0 = lambda(x: T)t` and the last rule is
+**Case (All-I)** Then `t0 = λ(x: T)t` and the last rule is
 
-                     G, x0: S0, G', x: T |- t: U
+                     Γ, x0: S0, Γ', x: T ⊢ t: U
               ------------------------------------------
-              G, x0: S0, G' |- lambda(x: T)t: all(x: T)U
+              Γ, x0: S0, Γ' ⊢ λ(x: T)t: ∀(x: T)U
 
-By the I.H., `G, [s]G', [s]x: [s]T |- [s]t: [s]U`.
-By (All-I), `G, [s]G' |- lambda([s]x: [s]T)[s]t): all([s]x: [s]T)[s]U`.
-By applying Lemma (Renaming) twice to the RHS, `G, [s]G' |- [s]lambda(x: T)t): [s]all(x: T)U`.
+By the I.H., `Γ, [s]Γ', [s]x: [s]T ⊢ [s]t: [s]U`.
+By (All-I), `Γ, [s]Γ' ⊢ λ([s]x: [s]T)[s]t): ∀([s]x: [s]T)[s]U`.
+By applying Lemma (Renaming) twice to the RHS, `Γ, [s]Γ' ⊢ [s]λ(x: T)t): [s]∀(x: T)U`.
 
 **Case (All-E)** Then `t0 = x y` and the last rule is
 
-       G, x0: S0, G' |- x: all(y: S)T    G, x0: S0, G' |- y: S
+       Γ, x0: S0, Γ' ⊢ x: ∀(y: S)T    Γ, x0: S0, Γ' ⊢ y: S
        -------------------------------------------------------
-                    G, x0: S0, G' |- x y: [z:=y]T
+                    Γ, x0: S0, Γ' ⊢ x y: [z:=y]T
 
-By the. I.H., `G, [s]G' |- [s]x: all(z: [s]S)[s]T` and `G, [s]G' |- [s]y: [s]S`.
-By (All-E), `G, [s]G' |- [s]x [s]y: [z:=[s]y][s]T`.
+By the. I.H., `Γ, [s]Γ' ⊢ [s]x: ∀(z: [s]S)[s]T` and `Γ, [s]Γ' ⊢ [s]y: [s]S`.
+By (All-E), `Γ, [s]Γ' ⊢ [s]x [s]y: [z:=[s]y][s]T`.
 W.l.o.g choose `z` so that `z != x0`, `z != y`.
 Hence, `[z:=[s]z][s]` = [s][z:=y]. Together,
-`G,[s]G' |- [s](x y): [s][z:=y]T`.
+`Γ,[s]Γ' ⊢ [s](x y): [s][z:=y]T`.
 
 **Case ({}-I)**: Then `t0 = new(x: T)d` and the last rule is
 
-                     G, x0: S0, G', x: T |- d: T
+                     Γ, x0: S0, Γ', x: T ⊢ d: T
                 --------------------------------------
-                G, x0: S0, G' |- new(x: T)d: rec(x: T)
+                Γ, x0: S0, Γ' ⊢ new(x: T)d: μ(x: T)
 
-By the I.H., `G, [s]G', [s]x: [s]T |- [s]d: [s]T`.
-By ({}-I), `G, [s]G' |- new([s]x: [s]T)[s]d: rec([s]x: [s]T)`
+By the I.H., `Γ, [s]Γ', [s]x: [s]T ⊢ [s]d: [s]T`.
+By ({}-I), `Γ, [s]Γ' ⊢ new([s]x: [s]T)[s]d: μ([s]x: [s]T)`
 By applying Lemma (Renaming) twice to the RHS,
-`G, [s]G' |- [s]new(x: T)d: [s]rec(x: T)`.
+`Γ, [s]Γ' ⊢ [s]new(x: T)d: [s]μ(x: T)`.
 
 **Case ({}-E)** Then `t0 = x.a` and the last rule is:
 
-                     G, x0: S0, G' |- x: {a: T}
+                     Γ, x0: S0, Γ' ⊢ x: {a: T}
                      ---------------------------
-                       G, x0: S0, G' |- x.a: T
+                       Γ, x0: S0, Γ' ⊢ x.a: T
 
-By the I.H., `G, [s]G' |- [s]x: {a: [s]T}`.
-By ({}-E), `G, [s]G' |- [s]x.a: [s]T`.
+By the I.H., `Γ, [s]Γ' ⊢ [s]x: {a: [s]T}`.
+By ({}-E), `Γ, [s]Γ' ⊢ [s]x.a: [s]T`.
 
 **Case (Let)**: Then `t0 = let x = t in u` and the last rule is:
 
-    G, x0: S0, G' |- t: T   G, x0: S0, G', x: T |- u: U   (x not in fv(U))
+    Γ, x0: S0, Γ' ⊢ t: T   Γ, x0: S0, Γ', x: T ⊢ u: U   (x ∉ fv(U))
     ----------------------------------------------------------------------
-                      G, x0: S0, G' |- let x = t in u: U
+                      Γ, x0: S0, Γ' ⊢ let x = t in u: U
 
-By the I.H., `G, [s]G' |- [s]t: [s]T` and `G, [s]G', [s]x: [s]T |- [s]u: [s]U`.
-With (Let) it follows that `G, [s]G' |- let [s]x = [s]t in [s]u: [s]U`.
-By (Renaming), `G, [s]G' |- [s]let x = t in u: [s]U`.
+By the I.H., `Γ, [s]Γ' ⊢ [s]t: [s]T` and `Γ, [s]Γ', [s]x: [s]T ⊢ [s]u: [s]U`.
+With (Let) it follows that `Γ, [s]Γ' ⊢ let [s]x = [s]t in [s]u: [s]U`.
+By (Renaming), `Γ, [s]Γ' ⊢ [s]let x = t in u: [s]U`.
 
 **Case (Rec-I)**: Then `t0 = x` and the last rule is:
 
-                              G |- x: T
+                              Γ ⊢ x: T
                           -----------------
-                          G |- x: rec(x: T)
+                          Γ ⊢ x: μ(x: T)
 
-By the I.H., `G, [s]G' |- [s]x: [s]T`.
-By (Rec-I), `G, [s]G' |- [s]x: rec([s]x: [s]T)`.
-By applying Lemma (Renaming) to the `rec` term, `G, [s]G' |- [s]x: [s]rec(x: T)`.
+By the I.H., `Γ, [s]Γ' ⊢ [s]x: [s]T`.
+By (Rec-I), `Γ, [s]Γ' ⊢ [s]x: μ([s]x: [s]T)`.
+By applying Lemma (Renaming) to the `rec` term, `Γ, [s]Γ' ⊢ [s]x: [s]μ(x: T)`.
 
 **Case (Rec-E)**: Then `t0 = x` and the last rule is:
 
-                    G, x0: S0, G' |- x: rec(x: T)
+                    Γ, x0: S0, Γ' ⊢ x: μ(x: T)
                     -----------------------------
-                        G, x0: S0, G' |- x: T
+                        Γ, x0: S0, Γ' ⊢ x: T
 
-By the I.H., `G, [s]G' |- [s]x: [s]rec(x: T)`.
-By applying Lemma (Renaming) to the `rec` term, `G, [s]G' |- [s]x: rec([s]x: [s]T)`.
-By (Rec-E), `G, [s]G' |- [s]x: [s]T`.
+By the I.H., `Γ, [s]Γ' ⊢ [s]x: [s]μ(x: T)`.
+By applying Lemma (Renaming) to the `rec` term, `Γ, [s]Γ' ⊢ [s]x: μ([s]x: [s]T)`.
+By (Rec-E), `Γ, [s]Γ' ⊢ [s]x: [s]T`.
 
 **Case (&=I)**. Then `t0 = x` amd the last rule is:
 
-                        G |- x: T   G |- x: U
+                        Γ ⊢ x: T   Γ ⊢ x: U
                         ---------------------
-                            G |- x: T & U
+                            Γ ⊢ x: T & U
 
-By the I.H., `G, [s]G' |- [s]x: [s]T` and `G, [s]G' |- [s]x: [s]U`.
-By (&=I), `G, [s]G' |- [s]x: [s]T & [s]U`.
+By the I.H., `Γ, [s]Γ' ⊢ [s]x: [s]T` and `Γ, [s]Γ' ⊢ [s]x: [s]U`.
+By (&=I), `Γ, [s]Γ' ⊢ [s]x: [s]T & [s]U`.
 
 **Case (Sub)** Then `t0 = t` and the last rule is:
 
-           G, x0: S0, G' |- t: T   G, x0: S0, G' |- T <: U
+           Γ, x0: S0, Γ' ⊢ t: T   Γ, x0: S0, Γ' ⊢ T <: U
            -----------------------------------------------
-                        G, x0: S0, G' |- t: U
+                        Γ, x0: S0, Γ' ⊢ t: U
 
-By the I.H., `G, [s]G' |- [s]t: [s]T`.
-By (Subst-<:), `G, [s]G' |- [s]T <: [s]U`.
-By (Sub), `G, [s]G' |- [s]T: [s]U`.
+By the I.H., `Γ, [s]Γ' ⊢ [s]t: [s]T`.
+By (Subst-<:), `Γ, [s]Γ' ⊢ [s]T <: [s]U`.
+By (Sub), `Γ, [s]Γ' ⊢ [s]T: [s]U`.
 
 **Case (Fld)**. Then `t0 = {a = t}` and the last rule is:
 
-                        G, x0: S0, G' |- t: S
+                        Γ, x0: S0, Γ' ⊢ t: S
                    --------------------------------
-                   G, x0: S0, G' |- {a = t}: {a: T}
+                   Γ, x0: S0, Γ' ⊢ {a = t}: {a: T}
 
-By the I.H, `G, [s]G' |- [s]t: [s]S`.
-By (Fld), `G, [s]G' |- {a = [s]t}: {a: [s]T}`.
-Rewriting this gives `G, [s]G' |- [s]{a = t}: [s]{a: T}`.
+By the I.H, `Γ, [s]Γ' ⊢ [s]t: [s]S`.
+By (Fld), `Γ, [s]Γ' ⊢ {a = [s]t}: {a: [s]T}`.
+Rewriting this gives `Γ, [s]Γ' ⊢ [s]{a = t}: [s]{a: T}`.
 
 **Cases (Typ), (And)** are analogous to (Fld).
 
@@ -531,163 +531,163 @@ Rewriting this gives `G, [s]G' |- [s]{a = t}: [s]{a: T}`.
 
 ### Lemma (Subst-<:)
 
-If `G, x: S, G' |- T <: U` and
-`G, [x:=y]G' |- y: [x:=y]S`, then
-`G, [x:=y]G' |- [x:=y]T <: [x:=y]U`.
+If `Γ, x: S, Γ' ⊢ T <: U` and
+`Γ, [x:=y]Γ' ⊢ y: [x:=y]S`, then
+`Γ, [x:=y]Γ' ⊢ [x:=y]T <: [x:=y]U`.
 
 Proof by mutual induction on derivations.
 Let [s] = [x0:=y0].
-Assume `G, x0: S0, G' |- T0 <: U0` and `G, [s]G' |- y0: [s]S0`.
-To show: `G [s]G' |- [s]T0 <: [s]U0`.
+Assume `Γ, x0: S0, Γ' ⊢ T0 <: U0` and `Γ, [s]Γ' ⊢ y0: [s]S0`.
+To show: `Γ [s]Γ' ⊢ [s]T0 <: [s]U0`.
 
 We only show two cases; the others are similar.
 
 **Case(<:-Sel)**: Then `T0 = S` and the last rule of `D` is:
 
-                    G, x0: S0, G' |- x: {A: S..T}
+                    Γ, x0: S0, Γ' ⊢ x: {A: S..T}
                     -----------------------------
-                      G, x0: S0, G' |- S <: x.A
+                      Γ, x0: S0, Γ' ⊢ S <: x.A
 
-By the I.H., `G, [s]G' |- [s]x: {A: [s]S..[s]T}`.
-By (<:-Sel), `G, [s]G' |- [s]S <: [s]x.A`.
+By the I.H., `Γ, [s]Γ' ⊢ [s]x: {A: [s]S..[s]T}`.
+By (<:-Sel), `Γ, [s]Γ' ⊢ [s]S <: [s]x.A`.
 
-**Case (All-<:-All)** Then `T0 = all(x: S1)T1` and the last rule is:
+**Case (All-<:-All)** Then `T0 = ∀(x: S1)T1` and the last rule is:
 
-     G, x0: S0, G' |- S2 <: S1   G, x0: S0, G', x: S2 |- T1 <: T2
+     Γ, x0: S0, Γ' ⊢ S2 <: S1   Γ, x0: S0, Γ', x: S2 ⊢ T1 <: T2
      ------------------------------------------------------------
-            G, x0: S0, G' |- all(x: S1)T1 <: all(x: S2)T2
+            Γ, x0: S0, Γ' ⊢ ∀(x: S1)T1 <: ∀(x: S2)T2
 
-By the I.H., `G, [s]G' |- [s]S2 <: [s]S1` and
-`G, [s]G', [s]x: [s]S2 |- [s]T1 <: [s]T2`.
-By (All-<:-All), `G, [s]G' |- all([s]x: [s]S1)[s]T1 <: all([s]x: [s]S1)[s]T1`.
-By (Renaming), `G, [s]G' |- [s]all(x: S1)T1 <: [s]all(x: S2)T2`.
+By the I.H., `Γ, [s]Γ' ⊢ [s]S2 <: [s]S1` and
+`Γ, [s]Γ', [s]x: [s]S2 ⊢ [s]T1 <: [s]T2`.
+By (All-<:-All), `Γ, [s]Γ' ⊢ ∀([s]x: [s]S1)[s]T1 <: ∀([s]x: [s]S1)[s]T1`.
+By (Renaming), `Γ, [s]Γ' ⊢ [s]∀(x: S1)T1 <: [s]∀(x: S2)T2`.
 
 
 ### Lemma (Corresponding Definition Types)
 
-If `G ~ s` and `s(x) = new(x: S)d` for some definitions `d = d1 & ... & dn` then
- 1. `x: rec(x: S) in G`.
+If `Γ ~ s` and `s(x) = new(x: S)d` for some definitions `d = d1 & ... & dn` then
+ 1. `x: μ(x: S) in Γ`.
  2. `S = S1 & ... & Sn` where for each `i` either
 
-    - `di` is of the form `{a = t}` and `Si = {a: T}` for some `T` such that `G |- t: T`, or
+    - `di` is of the form `{a = t}` and `Si = {a: T}` for some `T` such that `Γ ⊢ t: T`, or
     - `di` is of the form `{A = T}` and `Si = {A: T..T}`.
 
-*Proof* By the definition of `~`, `G` contains a binding for `x`, say
-`G = G1,x:T,G2` such that `G1 |- s(x): T`. Also by the definition of `~` and with ({}-I),
-`G1 |-! new(x: S)d: rec(x: S)`, which establishes (1).
+*Proof* By the definition of `~`, `Γ` contains a binding for `x`, say
+`Γ = G1,x:T,G2` such that `G1 ⊢ s(x): T`. Also by the definition of `~` and with ({}-I),
+`G1 ⊢! new(x: S)d: μ(x: S)`, which establishes (1).
 Furthermore, by the formulation of the ({}-I) Rule and definition typing
 it follows that `S` has the form given in (2).
 
 ### Lemma (Corresponding types)
 
-If `G ~ s` and `x: T in G` then exactly one of the following alternatives applies:
- 1. `s(x) = lambda(y:S)t` for a term `t` such that `G, x: S |- t: U` and `T = all(x: S)U`.
- 2. `s(x) = new(s:S)d` and `T = rec(x:S)`.
+If `Γ ~ s` and `x: T in Γ` then exactly one of the following alternatives applies:
+ 1. `s(x) = λ(y:S)t` for a term `t` such that `Γ, x: S ⊢ t: U` and `T = ∀(x: S)U`.
+ 2. `s(x) = new(s:S)d` and `T = μ(x:S)`.
 
-*Proof*: Assume `x: T in G`, say `G = G1,x:T,G2`.
-By the definition of `~`, `G1 |-! v: T` for some value `v`.
+*Proof*: Assume `x: T in Γ`, say `Γ = G1,x:T,G2`.
+By the definition of `~`, `G1 ⊢! v: T` for some value `v`.
 We distinguish acccording to whether `v` is a `lambda` or `new`.
 
-In the first case, let `v = lambda(y: S)t`.
-By by definition of `|-!`, `T` is derived using rule (all-I).
-Hence, `T = all(x: S)U` for some type `U` such that `G1, x: S |- t: U`.
-By (Weakening), `G, x: S |- t: U`.
+In the first case, let `v = λ(y: S)t`.
+By by definition of `⊢!`, `T` is derived using rule (all-I).
+Hence, `T = ∀(x: S)U` for some type `U` such that `G1, x: S ⊢ t: U`.
+By (Weakening), `Γ, x: S ⊢ t: U`.
 
 In the second case, let `v = new(x: S)d`
 (arranging w.l.o.g by alpha renaming that the bound variable in the new is `x`).
-By by definition of `|-!`, `T` is derived using rule ({}-I).
-Hence, `T = rec(x: S)`.
+By by definition of `⊢!`, `T` is derived using rule ({}-I).
+Hence, `T = μ(x: S)`.
 
 ### Lemma (Unique tight bounds)
 
-If `G ~ s` and `G |-! x: {A: T1..T1}` and `G |-! x: {A: T2..T2}` then `T1 = T2`.
+If `Γ ~ s` and `Γ ⊢! x: {A: T1..T1}` and `Γ ⊢! x: {A: T2..T2}` then `T1 = T2`.
 
 *Proof*
-Since `G |-! x: {A: Ti..Ti}` (i = 1,2), `G` contains a binding for `x`, say `x: T in G`.
+Since `Γ ⊢! x: {A: Ti..Ti}` (i = 1,2), `Γ` contains a binding for `x`, say `x: T in Γ`.
 By (Corresponding Types) one of the following alternatives applies.
 
- 1. `s(x) = lambda(y:S)t` for a term `t` such that `G, x: S |- t: U` and `T = all(x: S)U`.
-    But `x: {A: Ti..Ti)` cannot be derived from `x: all(x: S)U` using only (Rec-E) and
+ 1. `s(x) = λ(y:S)t` for a term `t` such that `Γ, x: S ⊢ t: U` and `T = ∀(x: S)U`.
+    But `x: {A: Ti..Ti)` cannot be derived from `x: ∀(x: S)U` using only (Rec-E) and
     (And-<:), (Trans) subsumption steps, so this alternative is impossible.
 
- 2. `s(x) = new(x:S)d` and `T = rec(x:S)`. By (Corresponding Definition Types),
+ 2. `s(x) = new(x:S)d` and `T = μ(x:S)`. By (Corresponding Definition Types),
     `T` is of the form
-    `rec(x: S1 & ... & Sn)` where exactly one `Si` defines a label `A`. Let `Si = {A: U..U}`.
+    `μ(x: S1 & ... & Sn)` where exactly one `Si` defines a label `A`. Let `Si = {A: U..U}`.
     It follows that `T1 = U = T2`.
 
 
 ### Definition (Tight bound typing)
 
-A typing or subtyping derivation is *tight* in environment `G` if
+A typing or subtyping derivation is *tight* in environment `Γ` if
 it only contains the following
-tight variants of (Sel-<:), (<:-Sel) when `G' = G`:
+tight variants of (Sel-<:), (<:-Sel) when `Γ' = Γ`:
 
     (<:-Sel-tight)
-                              G' |-! x: {A: T..T}
+                              Γ' ⊢! x: {A: T..T}
                               -------------------
-                                 G' |- T <: x.A
+                                 Γ' ⊢ T <: x.A
     (Sel-<:-tight)
-                              G' |-! x: {A: T..T}
+                              Γ' ⊢! x: {A: T..T}
                               -------------------
-                                 G' |- x.A <: T
+                                 Γ' ⊢ x.A <: T
 
-For environments that extend G, full (Sel-<:) and (<:-Sel) are permitted.
+For environments that extend Γ, full (Sel-<:) and (<:-Sel) are permitted.
 
-We write `G |-# t: T` if `G |- t: T` with a derivation that is tight in `G`.
+We write `Γ ⊢# t: T` if `Γ ⊢ t: T` with a derivation that is tight in `Γ`.
 
-We write `G |-# S <: U` if `G |- S <: U` with a derivation that is tight in `G`.
+We write `Γ ⊢# S <: U` if `Γ ⊢ S <: U` with a derivation that is tight in `Γ`.
 
 
 ### Definition (Has member)
 
 A variable `x` with type `T` has a member `A: S..U`
-in environment `G`, written `G |-# x: T has A: S..U`, if `G |-# x: T` and
+in environment `Γ`, written `Γ ⊢# x: T has A: S..U`, if `Γ ⊢# x: T` and
 the judgement is derivable by the following rules.
 
     (Refl-has)
-                        G |-# x: {A: S..U} has A: S..U
+                        Γ ⊢# x: {A: S..U} has A: S..U
     (&-has)
-                           G |-# x: T1 has A: S..U
+                           Γ ⊢# x: T1 has A: S..U
                          ----------------------------
-                         G |-# x: T1 & T2 has A: S..U
+                         Γ ⊢# x: T1 & T2 has A: S..U
 
-                           G |-# x: T2 has A: S..U
+                           Γ ⊢# x: T2 has A: S..U
                          ----------------------------
-                         G |-# x: T1 & T2 has A: S..U
+                         Γ ⊢# x: T1 & T2 has A: S..U
     (rec-has)
-                            G |-# x: T has A: S..U
+                            Γ ⊢# x: T has A: S..U
                         ------------------------------
-                        G |-# x: rec(x: T) has A: S..U
+                        Γ ⊢# x: μ(x: T) has A: S..U
     (sel-has)
-                G |-! y: {B: T'..T'}   G |-# x: T' has A: S..U
+                Γ ⊢! y: {B: T'..T'}   Γ ⊢# x: T' has A: S..U
                 ----------------------------------------------
-                           G |-# x: y.B has A: S..U
+                           Γ ⊢# x: y.B has A: S..U
     (Bot-has)
-                        G |-# x: Bot has A: S..U
+                        Γ ⊢# x: Bot has A: S..U
 
 ### Lemma (Has member inversion)
-If `G |- x: T has A: S..U` then one of the following cases applies:
+If `Γ ⊢ x: T has A: S..U` then one of the following cases applies:
 
  1. `T = {A: S..U}`.
- 2. `T = T1 & T2` and `G |-# x: T1 has A: S..U` or `G |-# x: T2 has A: S..U`.
- 3. `T = rec(x: T')` and `G |-# x: T' has A: S..U`.
+ 2. `T = T1 & T2` and `Γ ⊢# x: T1 has A: S..U` or `Γ ⊢# x: T2 has A: S..U`.
+ 3. `T = μ(x: T')` and `Γ ⊢# x: T' has A: S..U`.
  4. `T = y.B` and there exists a type `T'` such that
-    `G |-! y: {B: T'..T'}` and `G |-# x: T' has A: S..U`.
+    `Γ ⊢! y: {B: T'..T'}` and `Γ ⊢# x: T' has A: S..U`.
  5. `T = Bot`.
 
 *Proof:* Direct from the (Has member) rules.
 
 ### Lemma (Has member tightness)
 
-If `G ~ s` and `s(x) = new(x: T)d` and `G |-# x: rec(x: T) has A: S..U` then
+If `Γ ~ s` and `s(x) = new(x: T)d` and `Γ ⊢# x: μ(x: T) has A: S..U` then
 there is a type `T'` such that `S = T'` and `U = T'`.
 
 *Proof:* By inspection of definition typing.
 
 ### Lemma (Has member covariance)
-If `G ~ s`, `G |-# T1 <: T2` and `G |-# x: T1` and `G |-# x: T2 has A: S2..U2` then
-there exist types `S1`, `U1` such that `G |-# x: T1 has A: S1..U1`
-and `G |-# S2 <: S1` and `G |-# U1 <: U2`.
+If `Γ ~ s`, `Γ ⊢# T1 <: T2` and `Γ ⊢# x: T1` and `Γ ⊢# x: T2 has A: S2..U2` then
+there exist types `S1`, `U1` such that `Γ ⊢# x: T1 has A: S1..U1`
+and `Γ ⊢# S2 <: S1` and `Γ ⊢# U1 <: U2`.
 
 *Proof:* by induction on subtyping derivations.
 
@@ -699,175 +699,175 @@ and `G |-# S2 <: S1` and `G |-# U1 <: U2`.
 
 **Case (Trans-<:)**. Then the last rule is:
 
-                    G |-# T1 <: T3   G |-# T3 <: T2
+                    Γ ⊢# T1 <: T3   Γ ⊢# T3 <: T2
                     -------------------------------
-                            G |-# T1 <: T2
+                            Γ ⊢# T1 <: T2
 
-By subsumption, since `G |-# x: T1` we have also `G |-# x: T3`.
+By subsumption, since `Γ ⊢# x: T1` we have also `Γ ⊢# x: T3`.
 By the I.H. there exist types `S3`, `U3` such that
-`G |-# x: T3 has A: S3..U3` and `G |- S2 <: S3` and `G |- U3 <: U2`.
-By the I.H. again, `G |- x: T1 has A: S1..U1` with `G |- S3 <: S1` and `G |- U1 <: U3`.
-By (Trans-<:), `G |- S2 <: S1` and `G |- U1 <: U2`.
+`Γ ⊢# x: T3 has A: S3..U3` and `Γ ⊢ S2 <: S3` and `Γ ⊢ U3 <: U2`.
+By the I.H. again, `Γ ⊢ x: T1 has A: S1..U1` with `Γ ⊢ S3 <: S1` and `Γ ⊢ U1 <: U3`.
+By (Trans-<:), `Γ ⊢ S2 <: S1` and `Γ ⊢ U1 <: U2`.
 
-**Case (And-<:)**. Then the last rule is one of the axioms `G |-# T2 & U <: T2` or
-`G |-# U & T2 <: T2`. Assume the first, the second is analogous. By rule (has-&),
-`G |-# x: T2 & U has A: S2..U2`.
+**Case (And-<:)**. Then the last rule is one of the axioms `Γ ⊢# T2 & U <: T2` or
+`Γ ⊢# U & T2 <: T2`. Assume the first, the second is analogous. By rule (has-&),
+`Γ ⊢# x: T2 & U has A: S2..U2`.
 
 **Case (<:-And)**. Then `T2 = T21 & T22` and the last rule is:
 
-                  G |-# T1 <: T21   G |-# T1 <: T22
+                  Γ ⊢# T1 <: T21   Γ ⊢# T1 <: T22
                   ---------------------------------
-                        G |-# T1 <: T21 & T22
+                        Γ ⊢# T1 <: T21 & T22
 
-By (Has member inversion), there exists `i in {1,2}` such that `G |-# x: T2i has A: S2..U2`.
-By the I.H., `G |-# x: T1 has S2..U2`.
+By (Has member inversion), there exists `i in {1,2}` such that `Γ ⊢# x: T2i has A: S2..U2`.
+By the I.H., `Γ ⊢# x: T1 has S2..U2`.
 
 **Case (Fld-<:-Fld)**. Does not apply since `{a: U}` cannot appear in a `has` judgement.
 
 **Case (Typ-<:-Typ)**. Then `T1 = {A1: S1..U1}` and `T2 = {A2: S2'..U2'}`
 and the last rule is:
 
-                  G |-# S2' <: S1   G |-# U1 <: U2'
+                  Γ ⊢# S2' <: S1   Γ ⊢# U1 <: U2'
                   ----------------------------------
-                  G |-# {A: S1..U1} <: {A: S2'..U2'}
+                  Γ ⊢# {A: S1..U1} <: {A: S2'..U2'}
 
 By (Has member inversion) on `T2`, `S2' = S2` and `U2' = U2`.
-By definition of (Has member) on `T1`, `G |-# x: T1 has A: S1..U1`.
+By definition of (Has member) on `T1`, `Γ ⊢# x: T1 has A: S1..U1`.
 By inversion of the subtyping rule, the result follows.
 
 **Case (<:-Sel-tight)**. Then `T2 = y.B` and the last rule is:
 
-                         G |-! y: {B: T1..T1}
+                         Γ ⊢! y: {B: T1..T1}
                          -------------------
-                           G |-# T1 <: y.B
+                           Γ ⊢# T1 <: y.B
 
 By (has member inversion), there exists a type `T` such that
-`G |-! y: {B: T..T}` and `G |-# x: T has A: S2..U2`.
+`Γ ⊢! y: {B: T..T}` and `Γ ⊢# x: T has A: S2..U2`.
 By (Unique tight bounds), `T = T1`, which proves the case.
 
 
 **Case (Sel-<:-tight)**. Then `T1 = y.B` and the last rule is:
 
-                         G |-! y: {B: T2..T2}
+                         Γ ⊢! y: {B: T2..T2}
                          -------------------
-                           G |-# y.B <: T2
+                           Γ ⊢# y.B <: T2
 
 By definition of (Has member), case (sel-has), the result follows.
 
-**Case (All-<:-All)**. Does not apply since `all(x:S)T` cannot appear in a `has` judgement.
+**Case (All-<:-All)**. Does not apply since `∀(x:S)T` cannot appear in a `has` judgement.
 
 ### Lemma (Has member monotonicity)
 
-If `G ~ s` and `s(x) = new(x: T0)d` and
-`G |-# x: T has A: S..U` then there exists a type `T1` such that
-`G |-# x: rec(x: T0) has {A: T1..T1}`
-and `G |-# S <: T1` and `G |-# T1 <: U`.
+If `Γ ~ s` and `s(x) = new(x: T0)d` and
+`Γ ⊢# x: T has A: S..U` then there exists a type `T1` such that
+`Γ ⊢# x: μ(x: T0) has {A: T1..T1}`
+and `Γ ⊢# S <: T1` and `Γ ⊢# T1 <: U`.
 
-*Proof:* By induction of `G |-# x: T`.
+*Proof:* By induction of `Γ ⊢# x: T`.
 
 **Case (Var)**. Then the last rule is
 
-                         G, x: T, G' |- x: T
+                         Γ, x: T, Γ' ⊢ x: T
 
-Since `G ~ s`, `T = rec(x: T0)`. By (Has member tightness), there is a type `T1` such that
+Since `Γ ~ s`, `T = μ(x: T0)`. By (Has member tightness), there is a type `T1` such that
 `S = T1` and `U = T1`.
 
 **Case (Sub)**. Then the last rule is:
 
-                     G |-# x: T2   G |-# T2 <: T
+                     Γ ⊢# x: T2   Γ ⊢# T2 <: T
                      ---------------------------
-                              G |-# x: T
+                              Γ ⊢# x: T
 
 By (Has member covariance) there are types `S1`, `U1` such that
-`G |- x: T2 has A: S1..T1` and `G |- S <: S1` and `G |- U1 <: U`.
-By the I.H. there exists a type  `T1` such that `G |- x: rec(x: T0) has {A: T1..T1}`
-and `G |- S <: T1` and `G |- T1 <: U1`. By (Trans) `G |- S <: T1` and `G |- T1 <: U`.
+`Γ ⊢ x: T2 has A: S1..T1` and `Γ ⊢ S <: S1` and `Γ ⊢ U1 <: U`.
+By the I.H. there exists a type  `T1` such that `Γ ⊢ x: μ(x: T0) has {A: T1..T1}`
+and `Γ ⊢ S <: T1` and `Γ ⊢ T1 <: U1`. By (Trans) `Γ ⊢ S <: T1` and `Γ ⊢ T1 <: U`.
 
-**Case (Rec-I)**. Then `T = rec(x: T')` and the last rule is:
+**Case (Rec-I)**. Then `T = μ(x: T')` and the last rule is:
 
-                             G |-# x: T'
+                             Γ ⊢# x: T'
                           ------------------
-                         G |-# x: rec(x: T')
+                         Γ ⊢# x: μ(x: T')
 
-By (Has member inversion), `G |-# x: T' has A: S..U`.
+By (Has member inversion), `Γ ⊢# x: T' has A: S..U`.
 By the I.H., there exists a type `T1` such that
-`G |-# x: rec(x: T0) has {A: T1..T1}` and `G |-# S <: T1` and `G |-# T1 <: U`.
+`Γ ⊢# x: μ(x: T0) has {A: T1..T1}` and `Γ ⊢# S <: T1` and `Γ ⊢# T1 <: U`.
 
 **Case (Rec-E)**. Then the last rule is:
 
-                          G |-# x: rec(x: T)
+                          Γ ⊢# x: μ(x: T)
                           -----------------
-                              G |-# x: T
+                              Γ ⊢# x: T
 
-By (has-rec), `G |-# x: rec(x: T) has A: S..U`.
+By (has-rec), `Γ ⊢# x: μ(x: T) has A: S..U`.
 By the I.H. there exists a type `T1` such that
-`G |-# x: rec(x: T0) has {A: T1..T1}` and `G |-# S <: T1` and `G |-# T1 <: U`.
+`Γ ⊢# x: μ(x: T0) has {A: T1..T1}` and `Γ ⊢# S <: T1` and `Γ ⊢# T1 <: U`.
 
 **Case (&-I)**. Then `T = T1 & T2` and the last rule is:
 
-                      G |-# x: T1   G |-# x: T2
+                      Γ ⊢# x: T1   Γ ⊢# x: T2
                       -------------------------
-                           G |- x: T1 & T2
+                           Γ ⊢ x: T1 & T2
 
-By (Has member inversion), there exists `i in {1,2}` such that `G |-# x: Ti has A: S..U`.
-By the I.H. there exists a type  `T1` such that `G |- x: rec(x: T') has {A: T1..T1}`
-and `G |- S <: T1` and `G |- T1 <: U`.
+By (Has member inversion), there exists `i in {1,2}` such that `Γ ⊢# x: Ti has A: S..U`.
+By the I.H. there exists a type  `T1` such that `Γ ⊢ x: μ(x: T') has {A: T1..T1}`
+and `Γ ⊢ S <: T1` and `Γ ⊢ T1 <: U`.
 
 ### Lemma (Tight bound completeness)
 
-If `G ~ s` and `s(x) = new(x: T)d` and `G |-# x: {A: S..U}` then `G |-# x.A <: U` and `G |-# S <: x.A`.
+If `Γ ~ s` and `s(x) = new(x: T)d` and `Γ ⊢# x: {A: S..U}` then `Γ ⊢# x.A <: U` and `Γ ⊢# S <: x.A`.
 
-*Proof:* Since `G |-# x: {A: S..U}`, we have also `G |-# x: {A: S..U} has A: S..U`.
+*Proof:* Since `Γ ⊢# x: {A: S..U}`, we have also `Γ ⊢# x: {A: S..U} has A: S..U`.
 By (Has member monotonicity), there exists a type  `T1` such that
-`G |-# x: rec(x: T) has {A: T1..T1}` and `G |-# S <: T1` and `G |-# T1 <: U`.
-By (Has member inversion, case 3), `G |-# x: T has A: T1..T1`.
+`Γ ⊢# x: μ(x: T) has {A: T1..T1}` and `Γ ⊢# S <: T1` and `Γ ⊢# T1 <: U`.
+By (Has member inversion, case 3), `Γ ⊢# x: T has A: T1..T1`.
 By (Corresponding Definition Types) `T` is of the form `S1 & ... & Sn` where each
 `Si` is of the form `{A: Ti..Ti}` or `{a: Ti}`.
 By (Has member inversion, case 2), there must exist a `Si` such that
-`G |- x: Si has A: T1..T1`.
+`Γ ⊢ x: Si has A: T1..T1`.
 By (Has member inversion), `Si = {A: T1..T1}`.
-By Definition of (|-!), `G |-! x: {A: T1..T1}`.
+By Definition of (⊢!), `Γ ⊢! x: {A: T1..T1}`.
 By definition of (Sel-<:-tight) and (<:-Sel-tight),
-`G |-# x.A <: T1` and `G |-# T1 <: x.A`.
+`Γ ⊢# x.A <: T1` and `Γ ⊢# T1 <: x.A`.
 By (Trans)
-`G |-# x.A <: U` and `G |-# S <: x.A`.
+`Γ ⊢# x.A <: U` and `Γ ⊢# S <: x.A`.
 
 ### Lemma (All-I Inversion)
 
-If `G |-! lambda(x: S)t: U` then `U = all(x: S)T` for some type `T` such that
-`G, x: S |- t: T`.
+If `Γ ⊢! λ(x: S)t: U` then `U = ∀(x: S)T` for some type `T` such that
+`Γ, x: S ⊢ t: T`.
 
 ### Lemma ({}-I Inversion)
 
-If `G |-! new(x: T)(d1 & ... & dn): U` then `U = rec(x: T)` and `T` is of the form `S1 & ... & Sn`, where each `Si` corresponds to exactly one definition `di` in the following way:
+If `Γ ⊢! new(x: T)(d1 & ... & dn): U` then `U = μ(x: T)` and `T` is of the form `S1 & ... & Sn`, where each `Si` corresponds to exactly one definition `di` in the following way:
 
- - if `di = {a = t}` then `Si = {a: T'}` for some `T'` such that `G |- t: T'`.
+ - if `di = {a = t}` then `Si = {a: T'}` for some `T'` such that `Γ ⊢ t: T'`.
  - if `di = {A = T}` then `Si = {A: T..T}`.
 
 ### Definition (Possible types)
 
-For a variable `x`, value `v`, environment `G`, the set
-`Ts(G, x, v)` of possible types of `x` defined as `v` in `G` is the smallest set `SS` such that:
+For a variable `x`, value `v`, environment `Γ`, the set
+`Ts(Γ, x, v)` of possible types of `x` defined as `v` in `Γ` is the smallest set `SS` such that:
 
  1. If `v = new(x: T)d` then `T` in `SS`.
- 2. If `v = new(x: T)d` and `{a = t}` in `d` and `G |- t: T'` then `{a: T'} in SS`.
- 3. If `v = new(x: T)d` and `{A = T'}` in `d` and `G |- S <: T'`, `G |- T' <: U`
+ 2. If `v = new(x: T)d` and `{a = t}` in `d` and `Γ ⊢ t: T'` then `{a: T'} in SS`.
+ 3. If `v = new(x: T)d` and `{A = T'}` in `d` and `Γ ⊢ S <: T'`, `Γ ⊢ T' <: U`
    then `{A: S..U} in SS`.
- 4. If `v = lambda(x: S)t` and `G, x: S |- t: T` and
-    `G |- S' <: S` and `G, x: S' |- T <: T'` then `all(x: S')T' in SS`.
+ 4. If `v = λ(x: S)t` and `Γ, x: S ⊢ t: T` and
+    `Γ ⊢ S' <: S` and `Γ, x: S' ⊢ T <: T'` then `∀(x: S')T' in SS`.
  5. If `S1 in SS` and `S2 in SS` then `S1 & S2 in SS`.
- 6. If `S in SS` and `G |-! y: {A: S..S}` then `y.A in SS`.
- 7. If `T in SS` and then `rec(x: T) in SS`.
+ 6. If `S in SS` and `Γ ⊢! y: {A: S..S}` then `y.A in SS`.
+ 7. If `T in SS` and then `μ(x: T) in SS`.
  8. `Top` in `SS`.
 
 ### Lemma (Tight possible types closure)
-If `G ~ s` and `s(x) = v` then
-`Ts(G, x, v)` is closed wrt `G |-# _ <: _`.
+If `Γ ~ s` and `s(x) = v` then
+`Ts(Γ, x, v)` is closed wrt `Γ ⊢# _ <: _`.
 
-*Proof*: Let `SS = Ts(G, x, v)`. We show `SS` is closed wrt `G |-# _ <: _`.
+*Proof*: Let `SS = Ts(Γ, x, v)`. We show `SS` is closed wrt `Γ ⊢# _ <: _`.
 
-Assume `T0 in SS` and `G |- T0 <: U0`.
-We show `U0 in SS` by an induction on subtyping derivations of `G |-# T0 <: U0`.
+Assume `T0 in SS` and `Γ ⊢ T0 <: U0`.
+We show `U0 in SS` by an induction on subtyping derivations of `Γ ⊢# T0 <: U0`.
 
 **Case (<:-Top)**. Then `U0 = Top`. By (rule 8), `Top` in `SS`.
 
@@ -877,9 +877,9 @@ We show `U0 in SS` by an induction on subtyping derivations of `G |-# T0 <: U0`.
 
 **Case (Trans-<:)**. Then last last rule is:
 
-                          G |- T0 <: S   G |- S <: U0
+                          Γ ⊢ T0 <: S   Γ ⊢ S <: U0
                           ---------------------------
-                                 G |- T0 <: U0
+                                 Γ ⊢ T0 <: U0
 
 Then by the I.H. (twice), `S in SS` and `U0 in SS`.
 
@@ -891,155 +891,155 @@ rule (5) as often as necessary, `U0 in SS`.
 If `T0` is part of `SS` because of rule (5),
 `U0` and `S` must both be in `SS`.
 
-**Case (<:-And)**. Then `U0 = T & U` and `G |- T0 <: T`, `G |- T0 <: U`.
+**Case (<:-And)**. Then `U0 = T & U` and `Γ ⊢ T0 <: T`, `Γ ⊢ T0 <: U`.
 By the I.H. `T` and `U` are in `SS`. Hence, with rule (5), `U0 in SS`.
 
 **Case (Fld-<:-Fld)**. Then `T0 = {a: T1}` and `U0 = {a: U1}` for types `T1`, `U1` such that
-`G |- T1 <: U1`. The only way `T0` can be in `SS` is through rule (2),
-or rule (1) convertible to rule (2) by `G ~ s`. That is,
-`v = new(x: T)d` and `{a = t}` in `d` and `G |- t: T1`. Since `G |- T1 <: U1`
-we get with (Sub) that `G |- t: U1`. With rule (2), `U0 in SS`.
+`Γ ⊢ T1 <: U1`. The only way `T0` can be in `SS` is through rule (2),
+or rule (1) convertible to rule (2) by `Γ ~ s`. That is,
+`v = new(x: T)d` and `{a = t}` in `d` and `Γ ⊢ t: T1`. Since `Γ ⊢ T1 <: U1`
+we get with (Sub) that `Γ ⊢ t: U1`. With rule (2), `U0 in SS`.
 
 **Case (Typ-<:-Typ)** Then `T0 = {A: T1..T2}` and `U0 = {A: U1..U2}` for types
-`T1`, `T2`, `U1`, `U2` such that `G |- U1 <: T1` and `G |- T2 <: U2`.
+`T1`, `T2`, `U1`, `U2` such that `Γ ⊢ U1 <: T1` and `Γ ⊢ T2 <: U2`.
 The only way `T0` can be in `SS` is through rule (3) or rule (1) convertible to
-rule (3) by `G ~ s`. That is,
-`v = new(x: T)d` and `{A = T'}` in `d` and `G |- T1 <: T'`, `G |- T' <: T2`.
-With (Trans), `G |- U1 <: T'` and `G |- T' <: U2`. With rule (3), `U0 in SS`.
+rule (3) by `Γ ~ s`. That is,
+`v = new(x: T)d` and `{A = T'}` in `d` and `Γ ⊢ T1 <: T'`, `Γ ⊢ T' <: T2`.
+With (Trans), `Γ ⊢ U1 <: T'` and `Γ ⊢ T' <: U2`. With rule (3), `U0 in SS`.
 
-**Case (<:-Sel-tight)**. Then `U0 = y.A` for some `y` such that `G |-! y: {A: T0..T0}`.
+**Case (<:-Sel-tight)**. Then `U0 = y.A` for some `y` such that `Γ ⊢! y: {A: T0..T0}`.
 With rule (6), `U0 in SS`.
 
-**Case (Sel-<:-tight)** Then `T0 = y.A` for some `y` such that `G |-! y: {A: U0..U0}`.
+**Case (Sel-<:-tight)** Then `T0 = y.A` for some `y` such that `Γ ⊢! y: {A: U0..U0}`.
 The only way `y.A` can be in `SS` is through rule (6).
 That is, there is a type `S in SS` such that
-`G |-! y: {A: S..S}`. By (Unique tight bounds), `U0 = S`, hence `U0 in SS`.
+`Γ ⊢! y: {A: S..S}`. By (Unique tight bounds), `U0 = S`, hence `U0 in SS`.
 
-**Case (All-<:-All)**. Then `T0 = all(y: T1)T2` and `U0 = all(y: U1)U2`
-for some `T1`, `U1` such that `G |- U1 <: T1` and for some `T2`, `U2`
-such that `G, y: U1 |- T2 <: U2`. The only way `T0` can be in `SS` is
-through rule (4). That is, `v = lambda(x: T)d` and `G |- T1 <: T` and
-`G, x: T1 |- t: T2`. By (Narrowing), `G, x: U1 |- t: T2`. With (Sub),
-`G, x: U1 |- t: U2`. With (Trans), `G |- U1 <: T`. With rule (4),
-`all(x: U1)U2 in SS`.
+**Case (All-<:-All)**. Then `T0 = ∀(y: T1)T2` and `U0 = ∀(y: U1)U2`
+for some `T1`, `U1` such that `Γ ⊢ U1 <: T1` and for some `T2`, `U2`
+such that `Γ, y: U1 ⊢ T2 <: U2`. The only way `T0` can be in `SS` is
+through rule (4). That is, `v = λ(x: T)d` and `Γ ⊢ T1 <: T` and
+`Γ, x: T1 ⊢ t: T2`. By (Narrowing), `Γ, x: U1 ⊢ t: T2`. With (Sub),
+`Γ, x: U1 ⊢ t: U2`. With (Trans), `Γ ⊢ U1 <: T`. With rule (4),
+`∀(x: U1)U2 in SS`.
 
-This concludes the induction. Therefore, `SS` is closed wrt `G |-# _ <: _`.
+This concludes the induction. Therefore, `SS` is closed wrt `Γ ⊢# _ <: _`.
 
 ### Lemma (Possible types completeness for values)
 
-If `G ~ s` and `x = v in s` and  `G |-! v: T` then `T in Ts(G, x, v)`.
+If `Γ ~ s` and `x = v in s` and  `Γ ⊢! v: T` then `T in Ts(Γ, x, v)`.
 
 *Proof*. Assume first that `v = new(x: S)d`.
-By the definition `|-!`, the proof of `G |-! v: T` must end in a `{}-I` rule.
-By ({}-I Inversion), `T = rec(x: S)`. By rule (1) of (Possible Types), `S in Ts(G, x, v)`.
-By rule (7) of (Possible Types), `rec(x: S) in Ts(G, x, v)`.
+By the definition `⊢!`, the proof of `Γ ⊢! v: T` must end in a `{}-I` rule.
+By ({}-I Inversion), `T = μ(x: S)`. By rule (1) of (Possible Types), `S in Ts(Γ, x, v)`.
+By rule (7) of (Possible Types), `μ(x: S) in Ts(Γ, x, v)`.
 
-Assume now that `v = lambda(x: S)t`. By the definition `|-!`, the proof of `G |-! v: T` must end in a `All-I` rule. By (All-I Inversion),
-`U = all(x: S)T` for some type `T` such that `G, x: S |- t: T`.
-By rule (4) of (Possible Types), `all(x: S)T in Ts(G, x, v)`.
+Assume now that `v = λ(x: S)t`. By the definition `⊢!`, the proof of `Γ ⊢! v: T` must end in a `All-I` rule. By (All-I Inversion),
+`U = ∀(x: S)T` for some type `T` such that `Γ, x: S ⊢ t: T`.
+By rule (4) of (Possible Types), `∀(x: S)T in Ts(Γ, x, v)`.
 
 
 ### Lemma (Tight possible types completeness)
 
-If `G ~ s` and `x = v in s` and  `G |-# x: T` then `T in Ts(G, x, v)`.
+If `Γ ~ s` and `x = v in s` and  `Γ ⊢# x: T` then `T in Ts(Γ, x, v)`.
 
-*Proof*: By induction on the derivation of `G |-# x: T`. The derivation
-of `G |-# x: T` must end in one of the following cases:
+*Proof*: By induction on the derivation of `Γ ⊢# x: T`. The derivation
+of `Γ ⊢# x: T` must end in one of the following cases:
 
-**Case (Var)**. Since  `G ~ s`, `G` contains a binding `x: T` such that `G |-! v: T`.
-By (Possible types completeness for values), `T in Ts(G, x, v)`.
+**Case (Var)**. Since  `Γ ~ s`, `Γ` contains a binding `x: T` such that `Γ ⊢! v: T`.
+By (Possible types completeness for values), `T in Ts(Γ, x, v)`.
 
 **Case (Rec-I)**. Then the last rule is:
 
-                                  G |-# x: T
+                                  Γ ⊢# x: T
                               -----------------
-                              G |-# x: rec(x: T)
+                              Γ ⊢# x: μ(x: T)
 
-By the I.H., `T in Ts(G, x, v)`. By rule (7) of (Possible Types), `rec(x: T) in Ts(G, x, v)`.
+By the I.H., `T in Ts(Γ, x, v)`. By rule (7) of (Possible Types), `μ(x: T) in Ts(Γ, x, v)`.
 
 **Case (Rec-E)**. Then the last rule is:
 
-                              G |-# x: rec(x: T)
+                              Γ ⊢# x: μ(x: T)
                               -----------------
-                                  G |-# x: T
+                                  Γ ⊢# x: T
 
-By the I.H., `rec(x: T) in Ts(G, x, v)`. The only way a `rec` type can be in `Ts(G, x, v)` is through rule (7). Hence, `T in Ts(G, x, v)`.
+By the I.H., `μ(x: T) in Ts(Γ, x, v)`. The only way a `rec` type can be in `Ts(Γ, x, v)` is through rule (7). Hence, `T in Ts(Γ, x, v)`.
 
 **Case (&-I). Then the last rule is:
 
-                            G |-# x: T   G |-# x: U
+                            Γ ⊢# x: T   Γ ⊢# x: U
                             ---------------------
-                                G |-# x: T & U
+                                Γ ⊢# x: T & U
 
-By the I.H., `T in Ts(G, x, v)` and `U in Ts(G, x, v)`. By rule (5) of (Possible Types),
-`T & U in Ts(G, x, v)`.
+By the I.H., `T in Ts(Γ, x, v)` and `U in Ts(Γ, x, v)`. By rule (5) of (Possible Types),
+`T & U in Ts(Γ, x, v)`.
 
 **Case (Sub)**. Then the last rule is:
 
-                           G |-# x: T   G |-# T <: U
+                           Γ ⊢# x: T   Γ ⊢# T <: U
                            -----------------------
-                                  G |-# x: U
+                                  Γ ⊢# x: U
 
-By the I.H., `T in Ts(G, x, v)`. By (Tight possible types closure), `U in Ts(G, x, v)`.
+By the I.H., `T in Ts(Γ, x, v)`. By (Tight possible types closure), `U in Ts(Γ, x, v)`.
 
-### Lemma (Equivalence of `G |- ...` and `G |-# ...`)
+### Lemma (Equivalence of `Γ ⊢ ...` and `Γ ⊢# ...`)
 
-`G |-# ...` to `G |- ...` is straightforward by mutual induction on
+`Γ ⊢# ...` to `Γ ⊢ ...` is straightforward by mutual induction on
 typing and subtyping derivations.
 
-For `G |-# ...` to `G |- ...`, all cases are straightforward by mutual
+For `Γ ⊢# ...` to `Γ ⊢ ...`, all cases are straightforward by mutual
 induction except tightening subtyping of type selections. We can use
-(Tight bound completeness), provided we can show that `G |-# x :
+(Tight bound completeness), provided we can show that `Γ ⊢# x :
 {A:S..U}` implies that `s(x) = new(x: T)d` for some `T` and `d`, given
-also `G ~ s`. Since `G ~ s`, we know that `s(x) = v` for some
-`v`. By (Tight possible types completeness), `{A:S..U} in Ts(G, x,
+also `Γ ~ s`. Since `Γ ~ s`, we know that `s(x) = v` for some
+`v`. By (Tight possible types completeness), `{A:S..U} in Ts(Γ, x,
 v)`. By inversion, `v` must have of the form `new(x: T)d` for some `T`
 and `d`.
 
 ### Lemma (Possible types closure)
-If `G ~ s` and `s(x) = v` then `Ts(G, x, v)` is closed wrt `G |- _ <: _`.
+If `Γ ~ s` and `s(x) = v` then `Ts(Γ, x, v)` is closed wrt `Γ ⊢ _ <: _`.
 
-*Proof*: By (Tight possible types) and (Equivalence of `G |- _ <: _` and `G |-# _ <: _`).
+*Proof*: By (Tight possible types) and (Equivalence of `Γ ⊢ _ <: _` and `Γ ⊢# _ <: _`).
 
 ### Lemma (Possible types completeness)
 
-If `G ~ s` and `x = v in s` and  `G |- x: T` then `T in Ts(G, x, v)`.
+If `Γ ~ s` and `x = v in s` and  `Γ ⊢ x: T` then `T in Ts(Γ, x, v)`.
 
-*Proof*: By (Tight possible types completeness) and (Equivalence of `G |- _ : _` and `G |-# _ : _`).
+*Proof*: By (Tight possible types completeness) and (Equivalence of `Γ ⊢ _ : _` and `Γ ⊢# _ : _`).
 
 ### Lemma (Possible types)
-If `G ~ s` and `G |- x: T` then, for some value `v`,
-`s(x) = v` and `T in Ts(G, x, v)`.
+If `Γ ~ s` and `Γ ⊢ x: T` then, for some value `v`,
+`s(x) = v` and `T in Ts(Γ, x, v)`.
 
-*Proof*: If `G |- x: T`, `x` must be bound in `G`. Since `G ~ s` there must be a value `v`
-such that `s |= x = v`. By (Possible types completeness), `T in Ts(G, x, v)`.
+*Proof*: If `Γ ⊢ x: T`, `x` must be bound in `Γ`. Since `Γ ~ s` there must be a value `v`
+such that `s |= x = v`. By (Possible types completeness), `T in Ts(Γ, x, v)`.
 
 ### Lemma (Canonical forms 1)
-If `G ~ s` and `G |- x: all(x: T)U` then `s(x) = lambda(x: T')t` where
-`G |- T <: T'` and `G, x: T |- t: U`.
+If `Γ ~ s` and `Γ ⊢ x: ∀(x: T)U` then `s(x) = λ(x: T')t` where
+`Γ ⊢ T <: T'` and `Γ, x: T ⊢ t: U`.
 
-Proof: Since `x` has a type in `G`, `x` must be bound in `G`, say `G = G1,x:S,G2`.
-Since `G ~ s` there exists a value `v` such that `x = v` in `s` and `G1 |- v:S`.
-By (Possible Types), `v` cannot be a new because `all(x: T)U` is not in `T(G, x, v)`
+Proof: Since `x` has a type in `Γ`, `x` must be bound in `Γ`, say `Γ = G1,x:S,G2`.
+Since `Γ ~ s` there exists a value `v` such that `x = v` in `s` and `G1 ⊢ v:S`.
+By (Possible Types), `v` cannot be a new because `∀(x: T)U` is ∉ `T(Γ, x, v)`
 if `v` is a `new`.
-So `v` must be of the form `lambda(x: T')t`.
-Again by (Possible Types) the only way an `x` defined as a `lambda(x: T')t`
-can have a type `all(x: T)U` is
-if, for some `U0`, `G |- T <: T'`, `G, x: T' |- t: U0` and `G, x: T |- U0 <: U`.
-By (Sub) and (Narrowing), `G, x: T |- t: U`.
+So `v` must be of the form `λ(x: T')t`.
+Again by (Possible Types) the only way an `x` defined as a `λ(x: T')t`
+can have a type `∀(x: T)U` is
+if, for some `U0`, `Γ ⊢ T <: T'`, `Γ, x: T' ⊢ t: U0` and `Γ, x: T ⊢ U0 <: U`.
+By (Sub) and (Narrowing), `Γ, x: T ⊢ t: U`.
 
 ### Lemma (Canonical forms 2)
-If `G ~ s` and `G |- x: {a: T}` then `s(x) = new(x: S)d` for some type `S`,
+If `Γ ~ s` and `Γ ⊢ x: {a: T}` then `s(x) = new(x: S)d` for some type `S`,
 definition `d` such that
-`G |- d: S` and `d` contains a definition `{a = t}` where `G |- t: T`.
+`Γ ⊢ d: S` and `d` contains a definition `{a = t}` where `Γ ⊢ t: T`.
 
-Proof: Since `x` has a type in `G`, `x` must be bound in `G`, say `G = G1,x:S,G2`.
-Since `G ~ s` there exists a value `v` such that `x = v` in `s` and `G1 |- v:S`.
-By (Possible Types) `v` cannot be a lambda because `{a: T}` is not in `T(G, x, v)`
+Proof: Since `x` has a type in `Γ`, `x` must be bound in `Γ`, say `Γ = G1,x:S,G2`.
+Since `Γ ~ s` there exists a value `v` such that `x = v` in `s` and `G1 ⊢ v:S`.
+By (Possible Types) `v` cannot be a lambda because `{a: T}` is ∉ `T(Γ, x, v)`
 if `v` is a `lambda`.
 So `v` must be of the form `new(x: S)d`.
 Again by (Possible Types) the only way an `x` defined as `new(x: S)d` can have a type
-`{a: T}` is if there is a definition `{a = t}` in `d` and `G |- t: T`.
+`{a: T}` is if there is a definition `{a = t}` in `d` and `Γ ⊢ t: T`.
 
 
 <!---
@@ -1048,17 +1048,17 @@ Again by (Possible Types) the only way an `x` defined as `new(x: S)d` can have a
 Instead of (Ex-<:) and (<:-Ex) one may equivalently use the three rules below:
 
     (Ex-<:)
-                               (x not in fv(T))
+                               (x ∉ fv(T))
                              -------------------
-                             G |- ex(x: S)T <: T
+                             Γ ⊢ ex(x: S)T <: T
     (<:-Ex)
-                                  G |- x: S
+                                  Γ ⊢ x: S
                             ---------------------
-                             G |- T <: ex(x: S)T
+                             Γ ⊢ T <: ex(x: S)T
     (Ex-<:-Ex)
-                     G :- S1 <: S2   G, x: S1 |- T1 <: T2
+                     Γ :- S1 <: S2   Γ, x: S1 ⊢ T1 <: T2
                      ------------------------------------
-                       G |- ex(x: S1)T1 <: ex(x: S2)T2
+                       Γ ⊢ ex(x: S1)T1 <: ex(x: S2)T2
 
 Proof: we can derive each rule in one rule system using the rules of the other.
 -->
@@ -1066,57 +1066,57 @@ Proof: we can derive each rule in one rule system using the rules of the other.
 
 ### Theorem (Preservation)
 
-If `G |- t: T` and `G ~ s` and `s | t -> s' | t'`, then there exists
-an environment `G''` such that, letting `G' = G, G''` one has `G' |- t': T` and `G' ~ s'`.
+If `Γ ⊢ t: T` and `Γ ~ s` and `s | t -> s' | t'`, then there exists
+an environment `Γ''` such that, letting `Γ' = Γ, Γ''` one has `Γ' ⊢ t': T` and `Γ' ~ s'`.
 
 ### Theorem (Progress)
 
-If `G |- t: T` and `G ~ s` then either
+If `Γ ⊢ t: T` and `Γ ~ s` then either
 
  - `t` is a normal form, or
  - `s | t -> s' | t'`, for some store `s'`, term `t'`.
 
 *Proof*: We prove both theorems together. To be shown:
 
-Let `G |- t: T` and `G ~ s`. Then either
+Let `Γ ⊢ t: T` and `Γ ~ s`. Then either
 
  - `t` is a normal form, or
  - there exists a store `s'`, term `t'` such that `s | t -> s' | t'`, and
-   for any such `s'`, `t'` there exists an environment `G''` such that, letting `G' = G, G''` one has
-   `G' |- t': T` and `G' ~ s'`.
+   for any such `s'`, `t'` there exists an environment `Γ''` such that, letting `Γ' = Γ, Γ''` one has
+   `Γ' ⊢ t': T` and `Γ' ~ s'`.
 
-The proof is by a induction on typing derivations of `G |- t: T`.
+The proof is by a induction on typing derivations of `Γ ⊢ t: T`.
 
 If the last rule is one of (Var), (All-I), ({}-I), (Rec-I), (Rec-E), (&-I),
 `t` is a normal form and the result follows immediately.
 
 **Case (All-E)**: Then the last rule is:
 
-                       G |- x: all(z: S)T    G |- z: S
+                       Γ ⊢ x: ∀(z: S)T    Γ ⊢ z: S
                        -------------------------------
-                                 G |- x y: [z:=y]T
+                                 Γ ⊢ x y: [z:=y]T
 
-Since `G ~ s`, `G |- s(x): all(z: S)T`. By (Canonical forms 1),
-`s(x) = lambda(z: S')t` where `G |- S <: S'` and `G, z: S |- t: T`.
+Since `Γ ~ s`, `Γ ⊢ s(x): ∀(z: S)T`. By (Canonical forms 1),
+`s(x) = λ(z: S')t` where `Γ ⊢ S <: S'` and `Γ, z: S ⊢ t: T`.
 By (Apply), `s | x y ->  s | [z:=y]t`.
-By (Subst), G |- [z:=y]t: [z:=y]T.
+By (Subst), Γ ⊢ [z:=y]t: [z:=y]T.
 
 **Case ({}-E)**: Then the last rule is:
 
-                                G |- x: {a: T}
-                                --------------
-                                 G |- x.a: T
+                                Γ ⊢ x: {a: T}
+                                -------------
+                                 Γ ⊢ x.a: T
 
-Since `G ~ s`, `G |- s(x): {a: T}`. By (Canonical forms 2),
-`s(x) = new(y: S)d` for some binding `y = new(y: S)d`, such that `G |- d: S` and `d` contains
-a definition `{a = t}` where `G |- t: T`.
+Since `Γ ~ s`, `Γ ⊢ s(x): {a: T}`. By (Canonical forms 2),
+`s(x) = new(y: S)d` for some binding `y = new(y: S)d`, such that `Γ ⊢ d: S` and `d` contains
+a definition `{a = t}` where `Γ ⊢ t: T`.
 By (Project) `s | x.a -> s | t`, which proves the case.
 
 **Case (Let)**: Then the last rule is:
 
-                G |- t: T   G, x: T |- u: U   (x not in fv(U))
+                Γ ⊢ t: T   Γ, x: T ⊢ u: U   (x ∉ fv(U))
                 ----------------------------------------------
-                            G |- let x = t in u: U
+                            Γ ⊢ let x = t in u: U
 
 we distinguish according to whether `t` is a value, variable, or general term.
 
@@ -1129,37 +1129,37 @@ contain a ({}-I) rule, which can be only followed by subsumption
 steps. Let `T'` be the type obtained for `v` by the (All-I) or ({}-I)
 rule and let `D` be the (possibly empty) sequence of subsumption steps
 that follows it. Applying a (Var) step on `x` and following with `D`
-gives a derivation of `G, x: T' |- x: T`.
-This means `G, x: T' <: G, x: T`.
-By (Narrowing), `G, x: T' |- u: U`.
-Furthermore, by the construction of `T'`, `G |-! v: T'`, hence
-`G, x: T' ~ s, x = v`.
+gives a derivation of `Γ, x: T' ⊢ x: T`.
+This means `Γ, x: T' <: Γ, x: T`.
+By (Narrowing), `Γ, x: T' ⊢ u: U`.
+Furthermore, by the construction of `T'`, `Γ ⊢! v: T'`, hence
+`Γ, x: T' ~ s, x = v`.
 
 If `t = y` for some variable `y`, then by (Let-Var)
 `s | let x = y in t --> s | [x:=y]t`.
-The preconditions of the last rule are then: `G |- y: T` and `G, x: T |- u: U` and
-`x not in fv(U)`.
-Furthermore, since `fv(T) <= dom(G)` and `x not in dom(G)`, `x not in fv(T)`.
-It follows with (Subst) that `[x:=y]t: [x:=y]U`. Since `x not in fv(U)`, `[x:=y]U = U`,
+The preconditions of the last rule are then: `Γ ⊢ y: T` and `Γ, x: T ⊢ u: U` and
+`x ∉ fv(U)`.
+Furthermore, since `fv(T) <= dom(Γ)` and `x ∉ dom(Γ)`, `x ∉ fv(T)`.
+It follows with (Subst) that `[x:=y]t: [x:=y]U`. Since `x ∉ fv(U)`, `[x:=y]U = U`,
 which proves the case.
 
 If `t` is not a value nor a variable, then by the induction hypothesis
  there exist `s'`, `t'` such that `s | t -> s' | t'` and for any such
- `s'`, `t'` there exists an environment `G' = G, G''` such that `G' |-
- t': T` and `G' ~ s'`. By (Weakening) `G, G'', x: T |- u: U`. Hence,
- by (Let), `G' |- let x = t' in u: U`.
+ `s'`, `t'` there exists an environment `Γ' = Γ, Γ''` such that `Γ' ⊢
+ t': T` and `Γ' ~ s'`. By (Weakening) `Γ, Γ'', x: T ⊢ u: U`. Hence,
+ by (Let), `Γ' ⊢ let x = t' in u: U`.
 
 **Case (Sub)**: Then the last rule is:
 
-                           G |- t: T   G |- T <: U
+                           Γ ⊢ t: T   Γ ⊢ T <: U
                            -----------------------
-                                  G |- t: U
+                                  Γ ⊢ t: U
 
 If `t` is a value, the result follows immediately. Assume now that `t` is not a value.
 By the induction hypothesis there exist
  `s'`, `t'` such that `s | t -> s' | t'` and for any such `s'`, `t'`
- there exists an environment `G' = G, G''` such that `G' |- t': T` and
- `G' ~ s'`. By (Weakening, 2nd clause), `G' |- T <: U`.
-Then by (Sub) it follows that `G' |- t: U`.
+ there exists an environment `Γ' = Γ, Γ''` such that `Γ' ⊢ t': T` and
+ `Γ' ~ s'`. By (Weakening, 2nd clause), `Γ' ⊢ T <: U`.
+Then by (Sub) it follows that `Γ' ⊢ t: U`.
 
 
